transformations/DesugarScopedVarsImpl.dfy
@@ -114,11 +114,12 @@ module DesugarScopedVarsImpl {
     case _ => (c, counter) //TODO (precondition should eliminate this case)
   }   
 
-  function method RemoveScopedVarsAux(c: Cmd): (Cmd, seq<VarDecl>)
+  function method RemoveScopedVarsAux(c: Cmd): (res: (Cmd, seq<VarDecl>))
     /*requires substMap.Values <= set c,x | x in substMap.Keys && 0 < c < usedVars.1 :: VersionedName(x, c)
     requires forall x | x in substMap.Keys :: exists c : nat :: c <= usedVars.1 && substMap[x] == VersionedName(x, c)
     ensures 
       forall x | x in substMap.Keys :: exists c : nat :: c <= usedVars.1 && substMap[x] == VersionedName(x, c)*/
+    ensures NoScopedVars(res.0)
   {
     match c
     case SimpleCmd(sc) => (c, [])
@@ -130,12 +131,13 @@ module DesugarScopedVarsImpl {
     case Scope(optLabel, varDecls, body) =>
       var (body', declsBody) := RemoveScopedVarsAux(body);
       (Scope(optLabel, [], body'), varDecls + declsBody)
-    case If(None, thn, els) => 
-      //TODO: make sure If(Some(...)) has been desugared
+    case If(optGuard, thn, els) => 
       var (thn', declsThn) := RemoveScopedVarsAux(thn);
       var (els', declsEls) := RemoveScopedVarsAux(els);
-      (If(None, thn', els'), declsThn + declsEls)
-    case _ => (c, []) //TODO (precondition should eliminate this case)
+      (If(optGuard, thn', els'), declsThn + declsEls)
+    case Loop(invs, body) =>
+      var (body', declsBody) := RemoveScopedVarsAux(body);
+      (Loop(invs, body'), declsBody)
   }
 
   function method RemoveScopedVars(c: Cmd) : (Cmd, seq<VarDecl>)
@@ -186,14 +188,112 @@ module DesugarScopedVarsImpl {
     case Loop(_, body) => GetDecls(body)
   }
 
-  /** TODO */
-  /*
+  lemma AuxVersionedName(c1: nat, c2: nat, c3: nat)
+  ensures (iset i: nat, s: string | c1 <= i < c2 :: VersionedName(s, i)) !! (iset i: nat, s: string | c2 <= i < c3 :: VersionedName(s, i));
+  {
+    var xs := (iset i: nat, s: string | c1 <= i < c2 :: VersionedName(s, i));
+    var ys := (iset i: nat, s: string | c2 <= i < c3 :: VersionedName(s, i));
+    forall x | x in xs
+    ensures x !in ys
+    {
+      var i:nat,s :| x == VersionedName(s, i) && c1 <= i < c2;
+      forall y | y in ys
+      ensures x != y
+      {
+        var j:nat,s' :| y == VersionedName(s', j) && c2 <= j < c3;
+        assert VersionedName(s,i) != VersionedName(s',j) by {
+          VersionedNameInjective(s, s', i, j);
+        }
+      }
+    }
+  }
+
   lemma UniqueVars(c: Cmd, substMap: map<var_name, var_name>, counter: nat)
+    requires 
+      var (c',_) := MakeScopedVarsUnique(c, substMap, counter);
+      && NoLoopsNoIfGuard(c)
+      && NoLoopsNoIfGuard(c')
     ensures 
       var (c', counter') := MakeScopedVarsUnique(c, substMap, counter);
-      && Sequences.HasNoDuplicates(GetDecls(c'))
+      && Sequences.HasNoDuplicates(GetVarNamesSeq(GetDecls(c')))
+      && (iset s | s in GetVarNamesSeq(GetDecls(c'))) <= (iset i: nat, s: string | counter <= i < counter' :: VersionedName(s, i))
       && counter <= counter'
-  { assume false; }
-  */
+  { 
+    match c
+    case SimpleCmd(sc) =>   
+      reveal Sequences.HasNoDuplicates();
+    case Break(_) => 
+      reveal Sequences.HasNoDuplicates();
+    case Seq(c1, c2) => 
+      var (c1', counter1') := MakeScopedVarsUnique(c1, substMap, counter);
+      var (c2', counter2') := MakeScopedVarsUnique(c2, substMap, counter1');
+      AuxVersionedName(counter, counter1', counter2');
+
+      assert (iset i: nat, s: string | counter <= i < counter1' :: VersionedName(s, i)) !! (iset i: nat, s: string | counter1' <= i < counter2' :: VersionedName(s, i));
+
+      assert (set s | s in GetVarNamesSeq(GetDecls(c1'))) !! (set s | s in GetVarNamesSeq(GetDecls(c2')));
+        calc {
+          GetVarNamesSeq(GetDecls(Seq(c1',c2')));
+          GetVarNamesSeq(GetDecls(c1')+GetDecls(c2'));
+          GetVarNamesSeq(GetDecls(c1'))+GetVarNamesSeq(GetDecls(c2'));
+        }
+
+      assert Sequences.HasNoDuplicates(GetVarNamesSeq(GetDecls(c1'))+GetVarNamesSeq(GetDecls(c2'))) by {
+        AuxVersionedName(counter, counter1', counter2');
+        Util.HasNoDuplicatesAppDisj2(GetVarNamesSeq(GetDecls(c1')), GetVarNamesSeq(GetDecls(c2')));
+      }
+
+      var temp := (iset i: nat, s: string | counter <= i < counter2' :: VersionedName(s, i));
+      assert (iset s | s in GetVarNamesSeq(GetDecls(c1')))+(iset s | s in GetVarNamesSeq(GetDecls(c2'))) <= temp;
+    case Scope(optLabel, varDecls, body) =>
+      var varDecls' := CreateUniqueVarDecls(varDecls, counter);
+      var counter' := counter + |varDecls'|;
+      var substMap' := substMap + ConvertVDeclsToSubstMap(varDecls, varDecls');
+      var (body'', counter'') := MakeScopedVarsUnique(body, substMap', counter');
+
+      assert Sequences.HasNoDuplicates(GetVarNamesSeq(GetDecls(body'')));
+      assert Sequences.HasNoDuplicates(GetVarNamesSeq(varDecls')) by {
+        CreateUniqueVarDeclsNoDup(varDecls, counter);
+      }
+
+      var c' := Scope(optLabel, varDecls', body'');
+      calc {
+        GetVarNamesSeq(GetDecls(c'));
+        GetVarNamesSeq(varDecls'+GetDecls(body''));
+        GetVarNamesSeq(varDecls')+GetVarNamesSeq(GetDecls(body''));
+      }
+
+      assert Sequences.HasNoDuplicates(GetVarNamesSeq(varDecls')+GetVarNamesSeq(GetDecls(body''))) by {
+        AuxVersionedName(counter, counter', counter'');
+        Util.HasNoDuplicatesAppDisj2(GetVarNamesSeq(varDecls'), GetVarNamesSeq(GetDecls(body'')));
+      }
+
+      calc {
+        (iset s | s in GetVarNamesSeq(varDecls')+GetVarNamesSeq(GetDecls(body'')));
+        (iset s | s in GetVarNamesSeq(varDecls'))+(iset s | s in GetVarNamesSeq(GetDecls(body'')));
+      }
+    case If(None, thn, els) => 
+      var (thn', counter') := MakeScopedVarsUnique(thn, substMap, counter);
+      var (els', counter'') := MakeScopedVarsUnique(els, substMap, counter');
+      
+      assert Sequences.HasNoDuplicates(GetVarNamesSeq(GetDecls(thn')));
+      assert Sequences.HasNoDuplicates(GetVarNamesSeq(GetDecls(els')));
+
+      calc {
+        GetVarNamesSeq(GetDecls(If(None, thn', els')));
+        GetVarNamesSeq(GetDecls(thn')+GetDecls(els'));
+        GetVarNamesSeq(GetDecls(thn'))+GetVarNamesSeq(GetDecls(els'));
+      }
+  
+      assert Sequences.HasNoDuplicates(GetVarNamesSeq(GetDecls(thn'))+GetVarNamesSeq(GetDecls(els'))) by {
+        AuxVersionedName(counter, counter', counter'');
+        Util.HasNoDuplicatesAppDisj2(GetVarNamesSeq(GetDecls(thn')), GetVarNamesSeq(GetDecls(els')));
+      }
+
+      calc {
+        (iset s | s in GetVarNamesSeq(GetDecls(thn'))+GetVarNamesSeq(GetDecls(els')));
+        (iset s | s in GetVarNamesSeq(GetDecls(thn')))+(iset s | s in GetVarNamesSeq(GetDecls(els')));
+      }
+  }
 
 }
