util/ForallAppend.dfy
@@ -79,7 +79,7 @@ module ForallAppend {
           StateUpdVarDeclsSplit(s, d1[1..], d2, vs1[1..], vs2);
         }
         assert (d1+d2)[1..] == d1[1..]+d2 by {
-          SeqSliceAux(d1, d2); //DISCUSS (why can't Dafny prove the assertion without the helper lemma {:verify false}?)
+          SeqSliceAux(d1, d2); //DISCUSS (why can't Dafny prove the assertion without the helper lemma?)
         }
         assert (vs1+vs2)[1..] == vs1[1..]+vs2 by {
           SeqSliceAux(vs1, vs2);
@@ -105,6 +105,15 @@ module ForallAppend {
       { StateUpdVarDeclsSwap(s, d2, d1, vs2, vs1); }
       StateUpdVarDecls(StateUpdVarDecls(s, d1, vs1), d2, vs2);
     }
+  }
+
+  lemma StateUpdVarDeclsSplit3<A(!new)>(s: state<A>, d1: seq<VarDecl>, d2: seq<VarDecl>, vs1: seq<Val<A>>, vs2: seq<Val<A>>)
+    requires |d1| == |vs1| && |d2| == |vs2|
+    requires GetVarNames(d1) !! GetVarNames(d2)
+    ensures StateUpdVarDecls(s, d1+d2, vs1+vs2) == StateUpdVarDecls(s, d2+d1, vs2+vs1)
+  {
+    StateUpdVarDeclsSplit2(s, d1, d2, vs1, vs2);
+    StateUpdVarDeclsSplit(s, d2, d1, vs2, vs1);
   }
 
   lemma ValuesRespectDeclsSlice<A(!new)>(a: absval_interp<A>, vs: seq<Val<A>>, varDecls: seq<VarDecl>, start: nat, end: nat)
@@ -314,4 +323,149 @@ module ForallAppend {
         }
       }
     }
+  
+  lemma ValuesRespectDeclsAppendSwap<A(!new)>(a: absval_interp<A>, d1: seq<VarDecl>, d2: seq<VarDecl>, vs1: seq<Val<A>>, vs2: seq<Val<A>>)
+    requires 
+      && |vs1| == |d1|
+      && ValuesRespectDecls(a, vs1+vs2, d1+d2)
+    ensures
+      ValuesRespectDecls(a, vs2+vs1, d2+d1)
+  {
+    var vs := vs1+vs2;
+    var d := d1+d2;
+    var d' := d2+d1;
+
+    assert vs1 == vs[0..|d1|];
+    assert vs2 == vs[|d1|..|d|];
+
+    assert ValuesRespectDecls(a, vs1, d1) by {
+      ValuesRespectDeclsSlice(a, vs, d, 0, |d1|);
+    }
+
+    assert ValuesRespectDecls(a, vs2, d2) by {
+      ValuesRespectDeclsSlice(a, vs, d, |d1|, |d|);
+    }
+
+    assert ValuesRespectDecls(a, vs2+vs1, d') by {
+      ValuesRespectDeclsAppend(a, d2, d1, vs2, vs1);
+    }
+  }
+
+  lemma ForallVarDeclsSwap<A(!new)>(
+      a: absval_interp<A>, 
+      varDecls1: seq<(var_name, Ty)>, 
+      varDecls2: seq<(var_name, Ty)>, 
+      p: Predicate<A>,
+      s: state<A>)
+    requires GetVarNames(varDecls1) !! GetVarNames(varDecls2)
+    ensures    ForallVarDecls(a, varDecls1, ForallVarDecls(a, varDecls2, p))(s)
+            == ForallVarDecls(a, varDecls2, ForallVarDecls(a, varDecls1, p))(s)
+  {
+    calc {
+      ForallVarDecls(a, varDecls1, ForallVarDecls(a, varDecls2, p))(s);
+      { ForallVarDeclsAppend(a, varDecls1, varDecls2, p, s); }
+      ForallVarDecls(a, varDecls1+varDecls2, p)(s);
+      {  
+        if |varDecls1| == 0 || |varDecls2| == 0 {
+          var d := if |varDecls1| == 0 then varDecls2 else varDecls1;
+          assert varDecls1+varDecls2 == d == varDecls2+varDecls1;
+        } else {
+          var res1 := ForallVarDecls(a, varDecls1+varDecls2, p)(s);
+          var d := varDecls1+varDecls2;
+          var d' := varDecls2+varDecls1;
+
+          if res1 == None {
+            NoneForallVarDecls(a, d, p, s);
+            var vs :| ValuesRespectDecls(a, vs, d) && p(StateUpdVarDecls(s, d, vs)) == None;
+
+            var vs1 := vs[0..|varDecls1|];
+            var vs2 := vs[|varDecls1|..|d|];
+
+            assert vs == vs1+vs2;
+
+            assert ValuesRespectDecls(a, vs2+vs1, d') by {
+              ValuesRespectDeclsAppendSwap(a, varDecls1, varDecls2, vs1, vs2);
+            }
+
+            assert StateUpdVarDecls(s, d, vs) == StateUpdVarDecls(s, d', vs2+vs1) by {
+              StateUpdVarDeclsSplit3(s, varDecls1, varDecls2, vs1, vs2);
+            }
+
+            NoneForallVarDecls2(a, d', vs2+vs1, p, s);
+          } else if res1 == Some(true) {
+            forall vs | ValuesRespectDecls(a, vs, d')
+            ensures p(StateUpdVarDecls(s, d', vs)) == Some(true)
+            {
+              var vs2 := vs[0..|varDecls2|];
+              var vs1 := vs[|varDecls2|..|d|];
+
+              assert vs == vs2+vs1;
+
+              assert ValuesRespectDecls(a, vs1+vs2, d) by {
+                ValuesRespectDeclsAppendSwap(a, varDecls2, varDecls1, vs2, vs1);
+              }
+
+              assert StateUpdVarDecls(s, d', vs) == StateUpdVarDecls(s, d, vs1+vs2) by {
+                StateUpdVarDeclsSplit3(s, varDecls1, varDecls2, vs1, vs2);
+              }
+
+              SomeTrueForallVarDecls2(a, d, p, s, vs1+vs2);
+            }
+            SomeTrueForallVarDecls(a, d', p, s);
+          } else {
+            assert res1 == Some(false) by {
+              reveal ForallVarDecls();
+            }
+
+            forall vs | ValuesRespectDecls(a, vs, d')
+            ensures p(StateUpdVarDecls(s, d', vs)).Some?
+            {
+              var vs2 := vs[0..|varDecls2|];
+              var vs1 := vs[|varDecls2|..|d|];
+
+              assert vs == vs2+vs1;
+
+              assert ValuesRespectDecls(a, vs1+vs2, d) by {
+                ValuesRespectDeclsAppendSwap(a, varDecls2, varDecls1, vs2, vs1);
+              }
+
+              assert StateUpdVarDecls(s, d', vs) == StateUpdVarDecls(s, d, vs1+vs2) by {
+                StateUpdVarDeclsSplit3(s, varDecls1, varDecls2, vs1, vs2);
+              }
+
+              assert p(StateUpdVarDecls(s, d, vs1+vs2)).Some? by {
+                SomeForallVarDecls2(a, d, p, s, vs1+vs2);
+              }
+            }
+
+            assert ForallVarDecls(a, d', p)(s).Some? by {
+              SomeForallVarDecls3(a, d', p, s);
+            }
+
+            SomeFalseForallVarDecls2(a, d, p, s);
+
+            var vs :| ValuesRespectDecls(a, vs, d) && p(StateUpdVarDecls(s, d, vs)) == Some(false);
+            var vs1 := vs[0..|varDecls1|];
+            var vs2 := vs[|varDecls1|..|d|];
+
+            assert vs == vs1+vs2;
+
+            assert ValuesRespectDecls(a, vs2+vs1, d') by {
+              ValuesRespectDeclsAppendSwap(a, varDecls1, varDecls2, vs1, vs2);
+            }
+
+            assert StateUpdVarDecls(s, d, vs) == StateUpdVarDecls(s, d', vs2+vs1) by {
+              StateUpdVarDeclsSplit3(s, varDecls1, varDecls2, vs1, vs2);
+            }
+
+            SomeFalseForallVarDecls(a, d', p, s, vs2+vs1);
+          }
+        }
+      }
+      ForallVarDecls(a, varDecls2+varDecls1, p)(s);
+      { ForallVarDeclsAppend(a, varDecls2, varDecls1, p, s); }
+      ForallVarDecls(a, varDecls2, ForallVarDecls(a, varDecls1, p))(s);
+    }
+  }
+
 }
